Prove reader_prog semantics theorem
Also improve basis_ffi automation somewhat. But the main job here is
proving HOL_STORE_init_precond.

basis/basis_ffiLib.sig
@@ -4,6 +4,8 @@ signature basis_ffiLib = sig
 
   val add_basis_proj : thm -> thm
 
+  val hprop_heap_thms : thm list ref
+
   val call_thm : ml_progLib.ml_prog_state -> string -> thm -> thm * term
 
 end
